CollapsingTowers/TwoLvLBasic/Utils/Env.lean
@@ -1,4 +1,39 @@
 import CollapsingTowers.TwoLvLBasic.Syntax.Defs
+import CollapsingTowers.TwoLvLBasic.Utils.List
 
 abbrev TEnv :=
   List (Ty × Stage)
+
+@[simp]
+def escape : TEnv → TEnv
+  | [] => []
+  | (τ, .stat) :: tails => (τ, .stat) :: escape tails
+  | (τ, .dyn) :: tails => (τ, .stat) :: escape tails
+
+lemma escape.nil : [] = escape [] := by simp
+
+lemma escape.length : ∀ Γ, Γ.length = (escape Γ).length :=
+  by
+  intro Γ
+  induction Γ with
+  | nil => simp
+  | cons head _ IH =>
+    have ⟨τ, 𝕊⟩ := head
+    cases 𝕊 <;> (simp; apply IH)
+
+lemma binds.escape : ∀ Γ x τ 𝕊, binds x (τ, 𝕊) Γ → binds x (τ, .stat) (escape Γ) :=
+  by
+  intros Γ x τ 𝕊
+  induction Γ with
+  | nil => simp
+  | cons head tails IH =>
+    have ⟨τ, 𝕊⟩ := head
+    cases 𝕊
+    all_goals
+      simp
+      rw [← escape.length]
+      by_cases HEq : tails.length = x
+      . repeat rw [if_pos HEq]; simp
+        intros; assumption
+      . repeat rw [if_neg HEq]
+        apply IH
