CollapsingTowers/TwoLvLBasic/Semantic/Congruence.lean
@@ -1,6 +1,6 @@
 import CollapsingTowers.TwoLvLBasic.Semantic.SmallStep
 
-lemma pure_step.congruence_under_ctx𝔹 : ∀ B e₀ e₁, ctx𝔹 B → (e₀ ↦ e₁) → (B⟦e₀⟧ ↦ B⟦e₁⟧) :=
+lemma pure_step.congruence_under_ctx𝔹 : ∀ B e₀ e₁, ctx𝔹 B → (e₀ ⇾ e₁) → (B⟦e₀⟧ ⇾ B⟦e₁⟧) :=
   by
   intros B e₀ e₁ HB Hstep
   cases Hstep
@@ -10,7 +10,7 @@ lemma pure_step.congruence_under_ctx𝔹 : ∀ B e₀ e₁, ctx𝔹 B → (e₀ 
     apply ctx𝕄.cons𝔹; apply HB; apply HM
     apply Hlc; apply Hhead
 
-lemma pure_step.congruence_under_ctx𝔼 : ∀ E e₀ e₁, ctx𝔼 E → (e₀ ↦ e₁) → (E⟦e₀⟧ ↦ E⟦e₁⟧) :=
+lemma pure_step.congruence_under_ctx𝔼 : ∀ E e₀ e₁, ctx𝔼 E → (e₀ ⇾ e₁) → (E⟦e₀⟧ ⇾ E⟦e₁⟧) :=
   by
   intros E e₀ e₁ HE Hstep
   induction HE
@@ -19,7 +19,7 @@ lemma pure_step.congruence_under_ctx𝔼 : ∀ E e₀ e₁, ctx𝔼 E → (e₀ 
     simp; apply congruence_under_ctx𝔹
     apply HB; apply IH
 
-lemma pure_stepn.congruence_under_ctx𝔹 : ∀ B e₀ e₁, ctx𝔹 B → (e₀ ↦* e₁) → (B⟦e₀⟧ ↦* B⟦e₁⟧) :=
+lemma pure_stepn.congruence_under_ctx𝔹 : ∀ B e₀ e₁, ctx𝔹 B → (e₀ ⇾* e₁) → (B⟦e₀⟧ ⇾* B⟦e₁⟧) :=
   by
   intros B e₀ e₁ HB Hstepn
   induction Hstepn
@@ -29,7 +29,7 @@ lemma pure_stepn.congruence_under_ctx𝔹 : ∀ B e₀ e₁, ctx𝔹 B → (e₀
     apply pure_step.congruence_under_ctx𝔹
     apply HB; apply H; apply IH
 
-lemma pure_stepn.congruence_under_ctx𝔼 : ∀ E e₀ e₁, ctx𝔼 E → (e₀ ↦* e₁) → (E⟦e₀⟧ ↦* E⟦e₁⟧) :=
+lemma pure_stepn.congruence_under_ctx𝔼 : ∀ E e₀ e₁, ctx𝔼 E → (e₀ ⇾* e₁) → (E⟦e₀⟧ ⇾* E⟦e₁⟧) :=
   by
   intros E e₀ e₁ HE Hstepn
   induction Hstepn
