CollapsingTowers/TwoLvLBasic/SyntacticTyping/PresvHead.lean
@@ -1,0 +1,180 @@
+import CollapsingTowers.TwoLvLBasic.Semantic.Defs
+import CollapsingTowers.TwoLvLBasic.SyntacticTyping.PresvSubst
+import CollapsingTowers.TwoLvLBasic.SyntacticTyping.PresvMaping
+
+lemma typing.escape_strengthened :
+  ∀ Γ e τ,
+    typing Γ .dyn e τ ∅ →
+    typing (escape Γ) .stat e τ ∅ :=
+  by
+  generalize HEq𝕊 : (.dyn : Stage) = 𝕊
+  intros Γ e τ Hτ
+  apply
+    @typing.rec
+      (fun Γ 𝕊 e τ φ (H : typing Γ 𝕊 e τ φ) =>
+          .dyn = 𝕊 →
+          typing (escape Γ) .stat e τ φ)
+      (fun Γ e τ φ (H : typing_reification Γ e τ φ) => true)
+  <;> (intros; try contradiction)
+  case fvar x _ Hbinds HwellBinds HEq𝕊 =>
+    apply typing.fvar
+    apply binds.escape; apply Hbinds
+    apply wbt.escape; apply HwellBinds
+  case lam HwellBinds Hclose IH HEq𝕊 =>
+    rw [← HEq𝕊, escape] at IH
+    apply typing.lam; rw [← escape.length]
+    apply IH; rfl
+    apply wbt.escape; apply HwellBinds
+    rw [← escape.length]; apply Hclose
+  case app₁ IHf IHarg HEq𝕊 =>
+    apply typing.app₁
+    apply IHf; apply HEq𝕊
+    apply IHarg; apply HEq𝕊
+  case lit => apply typing.lit
+  case lets HwellBinds Hclose IHb IHe HEq𝕊 =>
+    rw [← HEq𝕊, escape] at IHe
+    apply typing.lets
+    apply IHb; apply HEq𝕊
+    rw [← escape.length]; apply IHe; rfl
+    apply wbt.escape; apply HwellBinds
+    rw [← escape.length]; apply Hclose
+  case pure => simp
+  case reify => simp
+  apply Hτ; apply HEq𝕊
+
+lemma typing.escape :
+  ∀ Γ e τ,
+    closed e →
+    typing Γ .dyn e τ ∅ →
+    typing Γ .stat e τ ∅ :=
+  by
+  intros Γ e τ Hclose Hτ
+  rw [← List.append_nil Γ]; apply typing.weakening
+  rw [escape.nil]; apply typing.escape_strengthened
+  induction Γ with
+  | nil => apply Hτ
+  | cons _ _ IH =>
+    apply IH
+    admit
+
+theorem preservation.head :
+  ∀ Γ e₀ e₁ τ φ,
+    head e₀ e₁ →
+    lc e₀ →
+    typing Γ .stat e₀ τ φ →
+    typing Γ .stat e₁ τ φ :=
+  by
+  intros Γ e₀ e₁ τ φ Hhead Hlc Hτ
+  cases Hhead
+  case lets Hvalue =>
+    cases Hτ
+    case lets e v τ φ _ _ Hτv Hclose Hτe =>
+      have Hpure : φ = (∅ : Effect) := by cases Hvalue <;> cases Hτv <;> rfl
+      rw [Hpure] at Hτv; simp [Hpure]
+      rw [← intros.subst]; apply preservation.subst
+      apply Hτv; apply Hτe; apply Hclose
+  case app₁ Hvalue =>
+    cases Hτ
+    case app₁ φ Hτv Hτf =>
+      cases Hτf
+      case lam Hclose _ Hτe =>
+        have Hpure : φ = (∅ : Effect) := by cases Hvalue <;> cases Hτv <;> rfl
+        rw [Hpure] at Hτv; simp [Hpure]
+        rw [← intros.subst]; apply preservation.subst
+        apply Hτv; apply Hτe; apply Hclose
+  case app₂ =>
+    cases Hτ
+    case app₂ Hτ₀ Hτ₁ =>
+      cases Hτ₀
+      case code_fragment HwellBinds₀ Hbinds₀ =>
+        cases Hτ₁
+        case code_fragment HwellBinds₁ Hbinds₁ =>
+          apply typing.reflect
+          rw [← union_pure_right ∅, ← union_pure_right (∅ ∪ ∅)]
+          apply typing.app₁
+          apply typing.fvar; apply Hbinds₀; apply HwellBinds₀
+          apply typing.fvar; apply Hbinds₁; apply HwellBinds₁
+  case lift_lit =>
+    cases Hτ
+    case lift_lit Hτ =>
+      apply typing.reflect
+      apply typing.lit
+    case lift_lam => contradiction
+  case lift_lam e =>
+    cases Hτ
+    case lift_lam Hτ =>
+      cases Hτ
+      case lam Hclose HwellBinds Hτe =>
+        rw [← intros.maping𝕔 Γ.length]
+        apply typing.lam𝕔
+        rw [identity.opening_closing]
+        apply typing_reification.reify
+        apply preservation.maping
+        apply Hτe
+        apply typing.code_fragment; simp
+        apply HwellBinds
+        apply lc.under_subst; simp
+        rw [lc.under_opening]; apply Hlc
+        apply HwellBinds
+        rw [← closed.under_closing]
+        apply closed.under_subst; simp
+        apply closed.under_opening; apply Hclose
+        apply Hclose
+    case lift_lit => contradiction
+  case lam𝕔 e =>
+    cases Hτ
+    case lam𝕔 HwellBinds Hτ Hclose =>
+      apply typing.reflect
+      apply typing.lam
+      cases Hτ with
+      | pure _ _ _ Hτ =>
+        simp at *
+        generalize Eqe : opening 0 (.fvar (List.length Γ)) e = E
+        rw [Eqe] at Hτ
+        cases Hτ with
+        | code_rep _ _ _ Hτ => apply Hτ
+      | reify _ _ _ _ Hτ =>
+        simp at *
+        generalize Eqe : opening 0 (.fvar (List.length Γ)) e = E
+        rw [Eqe] at Hτ
+        cases Hτ with
+        | code_fragment _ _ _ Hbinds HwellBinds =>
+          apply typing.fvar
+          apply Hbinds; apply HwellBinds
+      apply HwellBinds
+      apply Hclose
+  case lets𝕔 e =>
+    cases Hτ
+    case lets𝕔 HwellBinds Hτb Hτe Hclose =>
+      apply typing.code_rep
+      rw [← union_pure_right ∅]
+      apply typing.lets
+      apply Hτb
+      cases Hτe with
+      | pure _ _ _ Hτ =>
+        simp at *
+        generalize Eqe : ({0 ↦ (List.length Γ)} e) = E
+        rw [Eqe] at Hτ
+        cases Hτ with
+        | code_rep _ _ _ Hτ => apply Hτ
+      | reify _ _ _ _ Hτ =>
+        simp at *
+        generalize Eqe : opening 0 (.fvar (List.length Γ)) e = E
+        rw [Eqe] at Hτ
+        cases Hτ with
+        | code_fragment _ _ _ Hbinds HwellBinds =>
+          apply typing.fvar
+          apply Hbinds; apply HwellBinds
+      apply HwellBinds
+      apply Hclose
+  case run =>
+    cases Hτ
+    case run Hclose Hτ =>
+      cases Hτ with
+      | pure _ _ _ Hτ =>
+        cases Hτ
+        case code_rep Hτ =>
+          apply typing.escape
+          apply Hclose; apply Hτ
+      | reify _ _ _ _ Hτ =>
+        cases Hτ; contradiction
