CollapsingTowers/TwoLvLBasic/Syntax/Defs.lean
@@ -8,3 +8,4 @@ import CollapsingTowers.TwoLvLBasic.Syntax.Lc
 import CollapsingTowers.TwoLvLBasic.Syntax.Closed
 import CollapsingTowers.TwoLvLBasic.Syntax.Identity
 import CollapsingTowers.TwoLvLBasic.Syntax.Commutative
+import CollapsingTowers.TwoLvLBasic.Syntax.Intros
